bump example

theories/examples/delim_lang/glue.v
@@ -1089,248 +1089,248 @@ Proof.
   eauto with iFrame.
 Qed.
 
-(* Section faulty_glue. *)
-(*   Context {sz : nat}. *)
-(*   Variable rs : gReifiers CtxDep sz. *)
-(*   Context `{!subReifier reify_delim rs}. *)
-(*   Context `{!subReifier (sReifier_NotCtxDep_min reify_store CtxDep) rs}. *)
-(*   Notation F := (gReifiers_ops rs). *)
-(*   Context {R} `{!Cofe R}. *)
-(*   Context `{!SubOfe natO R}. *)
-(*   Context `{!SubOfe unitO R}. *)
-(*   Context `{!SubOfe locO R}. *)
-(*   Notation IT := (IT F R). *)
-(*   Notation ITV := (ITV F R). *)
+Section faulty_glue.
+  Context {sz : nat}.
+  Variable rs : gReifiers CtxDep sz.
+  Context `{!subReifier reify_delim rs}.
+  Context `{!subReifier (sReifier_NotCtxDep_min reify_store CtxDep) rs}.
+  Notation F := (gReifiers_ops rs).
+  Context {R} `{!Cofe R}.
+  Context `{!SubOfe natO R}.
+  Context `{!SubOfe unitO R}.
+  Context `{!SubOfe locO R}.
+  Notation IT := (IT F R).
+  Notation ITV := (ITV F R).
 
-(*   Context `{!invGS Σ, !stateG rs R Σ, !heapG rs R Σ}. *)
-(*   Notation iProp := (iProp Σ). *)
+  Context `{!invGS Σ, !stateG rs R Σ, !heapG rs R Σ}.
+  Notation iProp := (iProp Σ).
 
-(*   Program Fixpoint faulty_interp_expr {S} (e : expr S) : interp_scope S -n> IT := *)
-(*     match e with *)
-(*     | Var x => interp_var x *)
-(*     | App n m => interp_app rs (faulty_interp_expr n) (faulty_interp_expr m) *)
-(*     | LamV e => interp_lam rs (faulty_interp_expr e) *)
-(*     | NatOp op n m => interp_natop rs op (faulty_interp_expr n) (faulty_interp_expr m) *)
-(*     | Alloc e => interp_alloc rs (faulty_interp_expr e) *)
-(*     | Assign n m => interp_assign rs (faulty_interp_expr n) (faulty_interp_expr m) *)
-(*     | Deref e => interp_deref rs (faulty_interp_expr e) *)
-(*     | LocV l => interp_loc rs l *)
-(*     | UnitV => interp_unit rs *)
-(*     | LitV n => interp_nat rs n *)
-(*     | Embed e => constO $ (embed_lang.interp_closed  _ e) *)
-(*     end. *)
+  Program Fixpoint faulty_interp_expr {S} (e : expr S) : interp_scope S -n> IT :=
+    match e with
+    | Var x => interp_var x
+    | App n m => interp_app rs (faulty_interp_expr n) (faulty_interp_expr m)
+    | LamV e => interp_lam rs (faulty_interp_expr e)
+    | NatOp op n m => interp_natop rs op (faulty_interp_expr n) (faulty_interp_expr m)
+    | Alloc e => interp_alloc rs (faulty_interp_expr e)
+    | Assign n m => interp_assign rs (faulty_interp_expr n) (faulty_interp_expr m)
+    | Deref e => interp_deref rs (faulty_interp_expr e)
+    | LocV l => interp_loc rs l
+    | UnitV => interp_unit rs
+    | LitV n => interp_nat rs n
+    | Embed e => constO $ (embed_lang.interp_closed  _ e)
+    end.
 
-(*   Definition escape : embed_lang.expr ∅ := *)
-(*     ((shift/cc (($ 0) @k (# 42))))%syn. *)
+  Definition escape : embed_lang.expr ∅ :=
+    ((shift/cc (($ 0) @k (# 42))))%syn.
 
-(*   Definition buggy : expr ∅ *)
-(*     := App (LamV UnitV) (Alloc (Embed escape)). *)
+  Definition buggy : expr ∅
+    := App (LamV UnitV) (Alloc (Embed escape)).
 
-(*   Lemma typ_buggy : typed_glued □ buggy tUnit. *)
-(*   Proof. *)
-(*     repeat econstructor. *)
-(*   Qed. *)
+  Lemma typ_buggy : typed_glued □ buggy tUnit.
+  Proof.
+    repeat econstructor.
+  Qed.
 
-(*   Lemma faulty_spec_buggy : *)
-(*     ⊢ heap_ctx rs *)
-(*       -∗ has_substate ([] : delim.stateF ♯ IT) *)
-(*       -∗ WP@{rs} 𝒫 (faulty_interp_expr buggy ı_scope) @ notStuck *)
-(*            {{ βv, βv ≡ RetV () *)
-(*                   ∗ has_substate ([] : delim.stateF ♯ IT)}}. *)
-(*   Proof. *)
-(*     Opaque escape. *)
-(*     iIntros "T H". *)
-(*     cbn. *)
-(*     Transparent LET. *)
-(*     unfold LET. *)
-(*     simpl. *)
-(*     do 5 example.shift_hom. *)
-(*     iApply (wp_shift with "H"). *)
-(*     { rewrite laterO_map_Next. done. } *)
-(*     iIntros "!>_ H". *)
-(*     simpl. *)
-(*     rewrite get_val_ret. *)
-(*     simpl. *)
-(*     rewrite get_fun_fun. *)
-(*     simpl. *)
-(*     iApply (wp_app_cont with "H"). *)
-(*     { rewrite laterO_map_Next. done. } *)
-(*     iIntros "!>_ H". *)
-(*     simpl. *)
-(*     rewrite later_map_Next. *)
-(*     simpl. *)
-(*     rewrite <-Tick_eq. *)
-(*     iApply wp_tick. *)
-(*     iNext. *)
-(*     rewrite get_val_ret. *)
-(*     simpl.         *)
-(*     rewrite hom_vis. *)
-(*     match goal with *)
-(*     | |- context G [Vis _ _ ?a] => *)
-(*         set (k := a); *)
-(*         eassert (k ≡ NextO ◎ (_ ◎ (Ret ◎ (subEff_outs ^-1))))%stdpp as HEQ *)
-(*     end. *)
-(*     { *)
-(*       intro; simpl. *)
-(*       rewrite later_map_Next. *)
-(*       f_equiv. *)
-(*       reflexivity. *)
-(*     } *)
-(*     rewrite HEQ. *)
-(*     match goal with *)
-(*     | HEQ : (_ ≡ NextO ◎ ?a)%stdpp |- _ => *)
-(*         set (k' := a) *)
-(*     end. *)
-(*     match goal with *)
-(*     | |- context G [wp _ ?a] => *)
-(*         assert (a ≡ (ALLOC (Ret 42) (𝒫 ◎ k' ◎ subEff_outs)))%stdpp as -> *)
-(*     end. *)
-(*     { *)
-(*       Transparent ALLOC. *)
-(*       unfold ALLOC. *)
-(*       rewrite hom_vis. *)
-(*       simpl. *)
-(*       f_equiv; simpl. *)
-(*       intro; simpl. *)
-(*       rewrite later_map_Next. *)
-(*       do 4 (rewrite get_val_ITV; simpl). *)
-(*       do 2 (rewrite APP'_Fun_l; simpl). *)
-(*       reflexivity. *)
-(*     } *)
-(*     Opaque ALLOC. *)
-(*     simpl. *)
-(*     clear HEQ k. *)
-(*     iApply (wp_alloc with "T"); first solve_proper. *)
-(*     iIntros "!> !> %l Hl". *)
-(*     simpl. *)
-(*     rewrite get_val_ret. *)
-(*     simpl. *)
-(*     rewrite get_val_fun. *)
-(*     simpl. *)
-(*     rewrite APP'_Fun_l. *)
-(*     simpl. *)
-(*     rewrite <-Tick_eq. *)
-(*     rewrite hom_tick. *)
-(*     iApply wp_tick. *)
-(*     iNext. *)
-(*     iApply (wp_pop_cons with "H"). *)
-(*     iIntros "!> _ H". *)
-(*     iApply (wp_pop_end with "H"). *)
-(*     iIntros "!> _ H". *)
-(*     iApply wp_val. *)
-(*     iModIntro. *)
-(*     by iSplit. *)
-(*   Qed. *)
+  Lemma faulty_spec_buggy :
+    ⊢ heap_ctx rs
+      -∗ has_substate ([] : delim.stateF ♯ IT)
+      -∗ WP@{rs} 𝒫 (faulty_interp_expr buggy ı_scope) @ notStuck
+           {{ βv, βv ≡ RetV ()
+                  ∗ has_substate ([] : delim.stateF ♯ IT)}}.
+  Proof.
+    Opaque escape.
+    iIntros "T H".
+    cbn.
+    Transparent LET.
+    unfold LET.
+    simpl.
+    do 5 example.shift_hom.
+    iApply (wp_shift with "H").
+    { rewrite laterO_map_Next. done. }
+    iIntros "!>_ H".
+    simpl.
+    rewrite get_val_ret.
+    simpl.
+    rewrite get_fun_fun.
+    simpl.
+    iApply (wp_app_cont with "H").
+    { rewrite laterO_map_Next. done. }
+    iIntros "!>_ H".
+    simpl.
+    rewrite later_map_Next.
+    simpl.
+    rewrite <-Tick_eq.
+    iApply wp_tick.
+    iNext.
+    rewrite get_val_ret.
+    simpl.
+    rewrite hom_vis.
+    match goal with
+    | |- context G [Vis _ _ ?a] =>
+        set (k := a);
+        eassert (k ≡ NextO ◎ (_ ◎ (Ret ◎ (subEff_outs ^-1))))%stdpp as HEQ
+    end.
+    {
+      intro; simpl.
+      rewrite later_map_Next.
+      f_equiv.
+      reflexivity.
+    }
+    rewrite HEQ.
+    match goal with
+    | HEQ : (_ ≡ NextO ◎ ?a)%stdpp |- _ =>
+        set (k' := a)
+    end.
+    match goal with
+    | |- context G [wp _ ?a] =>
+        assert (a ≡ (ALLOC (Ret 42) (𝒫 ◎ k' ◎ subEff_outs)))%stdpp as ->
+    end.
+    {
+      Transparent ALLOC.
+      unfold ALLOC.
+      rewrite hom_vis.
+      simpl.
+      f_equiv; simpl.
+      intro; simpl.
+      rewrite later_map_Next.
+      do 4 (rewrite get_val_ITV; simpl).
+      do 2 (rewrite APP'_Fun_l; simpl).
+      reflexivity.
+    }
+    Opaque ALLOC.
+    simpl.
+    clear HEQ k.
+    iApply (wp_alloc with "T"); first solve_proper.
+    iIntros "!> !> %l Hl".
+    simpl.
+    rewrite get_val_ret.
+    simpl.
+    rewrite get_val_fun.
+    simpl.
+    rewrite APP'_Fun_l.
+    simpl.
+    rewrite <-Tick_eq.
+    rewrite hom_tick.
+    iApply wp_tick.
+    iNext.
+    iApply (wp_pop_cons with "H").
+    iIntros "!> _ H".
+    iApply (wp_pop_end with "H").
+    iIntros "!> _ H".
+    iApply wp_val.
+    iModIntro.
+    by iSplit.
+  Qed.
 
-(*   Lemma correct_spec_buggy : *)
-(*     ⊢ heap_ctx rs *)
-(*       -∗ has_substate ([] : delim.stateF ♯ IT) *)
-(*       -∗ WP@{rs} 𝒫 (interp_expr rs buggy ı_scope) @ notStuck *)
-(*            {{ βv, βv ≡ RetV () *)
-(*                   ∗ has_substate ([] : delim.stateF ♯ IT)}}. *)
-(*   Proof. *)
-(*     Opaque escape. *)
-(*     iIntros "T H". *)
-(*     cbn. *)
-(*     Transparent LET. *)
-(*     unfold LET. *)
-(*     simpl. *)
-(*     do 5 example.shift_hom. *)
-(*     iApply (wp_reset with "H"). *)
-(*     iIntros "!>_ H". *)
-(*     simpl. *)
-(*     unfold embed_lang.interp_closed. *)
-(*     simpl. *)
-(*     Transparent escape. *)
-(*     unfold escape. *)
-(*     simpl. *)
-(*     do 1 example.shift_hom. *)
-(*     (* iApply (wp_reset with "H"). *) *)
-(*     (* iIntros "!>_ H". *) *)
-(*     (* simpl. *) *)
-(*     (* do 1 example.shift_hom. *) *)
-(*     iApply (wp_shift with "H"). *)
-(*     { rewrite laterO_map_Next. done. } *)
-(*     iIntros "!>_ H". *)
-(*     simpl. *)
+  Lemma correct_spec_buggy :
+    ⊢ heap_ctx rs
+      -∗ has_substate ([] : delim.stateF ♯ IT)
+      -∗ WP@{rs} 𝒫 (interp_expr rs buggy ı_scope) @ notStuck
+           {{ βv, βv ≡ RetV ()
+                  ∗ has_substate ([] : delim.stateF ♯ IT)}}.
+  Proof.
+    Opaque escape.
+    iIntros "T H".
+    cbn.
+    Transparent LET.
+    unfold LET.
+    simpl.
+    do 5 example.shift_hom.
+    iApply (wp_reset with "H").
+    iIntros "!>_ H".
+    simpl.
+    unfold embed_lang.interp_closed.
+    simpl.
+    Transparent escape.
+    unfold escape.
+    simpl.
+    do 1 example.shift_hom.
+    (* iApply (wp_reset with "H"). *)
+    (* iIntros "!>_ H". *)
+    (* simpl. *)
+    (* do 1 example.shift_hom. *)
+    iApply (wp_shift with "H").
+    { rewrite laterO_map_Next. done. }
+    iIntros "!>_ H".
+    simpl.
 
-(*     rewrite get_val_ret. *)
-(*     simpl. *)
-(*     rewrite get_fun_fun. *)
-(*     simpl. *)
-(*     iApply (wp_app_cont with "H"). *)
-(*     { rewrite laterO_map_Next. done. } *)
-(*     iIntros "!>_ H". *)
-(*     simpl. *)
-(*     rewrite later_map_Next. *)
-(*     simpl. *)
-(*     rewrite <-Tick_eq. *)
-(*     iApply wp_tick. *)
-(*     iNext. *)
+    rewrite get_val_ret.
+    simpl.
+    rewrite get_fun_fun.
+    simpl.
+    iApply (wp_app_cont with "H").
+    { rewrite laterO_map_Next. done. }
+    iIntros "!>_ H".
+    simpl.
+    rewrite later_map_Next.
+    simpl.
+    rewrite <-Tick_eq.
+    iApply wp_tick.
+    iNext.
 
-(*     iApply (wp_pop_cons with "H"). *)
-(*     iIntros "!>_ H". *)
-(*     simpl. *)
-(*     iApply (wp_pop_cons with "H"). *)
-(*     iIntros "!> _ H". *)
-(*     simpl. *)
-(*     rewrite get_val_ret. *)
-(*     simpl. *)
-(*     simpl. *)
-(*     rewrite hom_vis. *)
-(*     match goal with *)
-(*     | |- context G [Vis _ _ ?a] => *)
-(*         set (k := a); *)
-(*         eassert (k ≡ NextO ◎ (_ ◎ (Ret ◎ (subEff_outs ^-1))))%stdpp as HEQ *)
-(*     end. *)
-(*     { *)
-(*       intro; simpl. *)
-(*       rewrite later_map_Next. *)
-(*       f_equiv. *)
-(*       reflexivity. *)
-(*     } *)
-(*     rewrite HEQ. *)
-(*     match goal with *)
-(*     | HEQ : (_ ≡ NextO ◎ ?a)%stdpp |- _ => *)
-(*         set (k' := a) *)
-(*     end. *)
-(*     match goal with *)
-(*     | |- context G [wp _ ?a] => *)
-(*         assert (a ≡ (ALLOC (Ret 42) (𝒫 ◎ k' ◎ subEff_outs)))%stdpp as -> *)
-(*     end. *)
-(*     { *)
-(*       Transparent ALLOC. *)
-(*       unfold ALLOC. *)
-(*       rewrite hom_vis. *)
-(*       simpl. *)
-(*       f_equiv; simpl. *)
-(*       intro; simpl. *)
-(*       rewrite later_map_Next. *)
-(*       do 4 (rewrite get_val_ITV; simpl). *)
-(*       do 2 (rewrite APP'_Fun_l; simpl). *)
-(*       reflexivity. *)
-(*     } *)
-(*     Opaque ALLOC. *)
-(*     simpl. *)
-(*     clear HEQ k. *)
-(*     iApply (wp_alloc with "T"); first solve_proper. *)
-(*     iIntros "!> !> %l Hl". *)
-(*     simpl. *)
-(*     rewrite get_val_ret. *)
-(*     simpl. *)
-(*     rewrite get_val_fun. *)
-(*     simpl. *)
-(*     rewrite APP'_Fun_l. *)
-(*     simpl. *)
-(*     rewrite <-Tick_eq. *)
-(*     rewrite hom_tick. *)
-(*     iApply wp_tick. *)
-(*     iNext. *)
-(*     iApply (wp_pop_end with "H"). *)
-(*     iIntros "!> _ H". *)
-(*     iApply wp_val. *)
-(*     iModIntro. *)
-(*     by iSplit. *)
-(*   Qed. *)
+    iApply (wp_pop_cons with "H").
+    iIntros "!>_ H".
+    simpl.
+    iApply (wp_pop_cons with "H").
+    iIntros "!> _ H".
+    simpl.
+    rewrite get_val_ret.
+    simpl.
+    simpl.
+    rewrite hom_vis.
+    match goal with
+    | |- context G [Vis _ _ ?a] =>
+        set (k := a);
+        eassert (k ≡ NextO ◎ (_ ◎ (Ret ◎ (subEff_outs ^-1))))%stdpp as HEQ
+    end.
+    {
+      intro; simpl.
+      rewrite later_map_Next.
+      f_equiv.
+      reflexivity.
+    }
+    rewrite HEQ.
+    match goal with
+    | HEQ : (_ ≡ NextO ◎ ?a)%stdpp |- _ =>
+        set (k' := a)
+    end.
+    match goal with
+    | |- context G [wp _ ?a] =>
+        assert (a ≡ (ALLOC (Ret 42) (𝒫 ◎ k' ◎ subEff_outs)))%stdpp as ->
+    end.
+    {
+      Transparent ALLOC.
+      unfold ALLOC.
+      rewrite hom_vis.
+      simpl.
+      f_equiv; simpl.
+      intro; simpl.
+      rewrite later_map_Next.
+      do 4 (rewrite get_val_ITV; simpl).
+      do 2 (rewrite APP'_Fun_l; simpl).
+      reflexivity.
+    }
+    Opaque ALLOC.
+    simpl.
+    clear HEQ k.
+    iApply (wp_alloc with "T"); first solve_proper.
+    iIntros "!> !> %l Hl".
+    simpl.
+    rewrite get_val_ret.
+    simpl.
+    rewrite get_val_fun.
+    simpl.
+    rewrite APP'_Fun_l.
+    simpl.
+    rewrite <-Tick_eq.
+    rewrite hom_tick.
+    iApply wp_tick.
+    iNext.
+    iApply (wp_pop_end with "H").
+    iIntros "!> _ H".
+    iApply wp_val.
+    iModIntro.
+    by iSplit.
+  Qed.
 
-(* End faulty_glue. *)
+End faulty_glue.
